compiler/dafny/semantics/README.md
@@ -15,5 +15,5 @@ Correctness proof for the freshen pass.
 [dafny_semanticPrimitivesScript.sml](dafny_semanticPrimitivesScript.sml):
 Defines semantic primitives used in Dafny's semantics.
 
-[evaluate_appsScript.sml](evaluate_appsScript.sml):
+[extension_evaluatePropsScript.sml](extension_evaluatePropsScript.sml):
 Properties of the operational semantics.
